FMT/API.lean
@@ -1,7 +1,14 @@
 import FMT.Types.LocalType
+import FMT.Types.Factorization
+import FMT.Bridge.LocalGlobal
 
 namespace FMT
 
-def useLocalType : FMT.Types.LocalType := FMT.Types.LocalType.one
+open FMT.Types
+
+def useLocalType : LocalType := LocalType.one
+
+def useLocalFactorization : FactorsThrough evalLocal FMT.Bridge.localProjection :=
+  FMT.Bridge.localToGlobal
 
 end FMT
